 \documentclass{article} \usepackage{amsmath} \usepackage{amssymb}  \begin{document}  93 r $ \lVert g_{i} \rVert^{2}N(\lVert g_{i} \rVert) $ $ \lvert H(Q_1,Q_2)^{2} - \lVert g_1 - g_2 \rVert^{2} \rvert \leq \lVert g_1 \rVert^{2} N(\lVert g_1 \rVert) + \lVert g_2 \rVert^{2} N(\lVert g_2 \rVert) $. If (6.2.3) holds for $ g_1 = q_i/p - 1 $, then the assumptions hold with $ r_i = 0 $, and we obtain $ \lvert H(Q_1,Q_2)^{2} - \Delta(Q_1,Q_2;P)^{2} \rvert \leq \Delta(Q_1;P)^{2} N(\Delta(Q_1;P)) $ + $ \Delta(Q_2;P)^{2} N(\Delta(Q_2;P)) $.  \textbf{Proof.} (i) In this proof, N denotes a generic null-function. Define $ A_i := \{ \lvert g_i \rvert \leq N(\lVert g_i \rVert) \}, \quad B_i := \{ \lvert r_i \rvert \leq 1 \}. $ By (6.2.3) and Lemma 19.1.1, (6.2.6) $ P(A_i^c) \leq \lVert g_i \rVert^{2} N(\lVert g_i \rVert) $ , (6.2.7) $ P(\lvert g_i \rvert 1_{A_i}^c) \leq \lVert g_i \rVert^{2} N(\lVert g_i \rVert) $ , (6.2.8) $ P(g_i^2 1_{A_i}^c) \leq \lVert g_i \rVert^{2} N(\lVert g_i \rVert) $.  From (6.2.4) and (6.2.5) we obtain (6.2.9) $ P(B_i^c) \leq \lVert g_i \rVert^{2} N(\lVert g_i \rVert) $ , (6.2.10) $ P(\lvert r_i \rvert 1_{B_i}^c) \leq \lVert g_i \rVert^{2} N(\lVert g_i \rVert) $ , (6.2.11) $ P(r_i^2 1_{B_i}) \leq \lVert g_i \rVert^{2} N(\lVert g_i \rVert) $.  We have $ H(Q_1,Q_2)^{2} = 8(1 - P(((1 + g_1 + r_1)(1 + g_2 + r_2))^{1/2})) $.  On D:= $ A_1 B_1 A_2 B_2 $ we obtain an expansion (6.2.12) $ ((1 + g_1 + r_1)(1 + g_2 + r_2))^{1/2} $ $ = 1 - \frac{1}{8} (g_1 - g_2)^{2} + \frac{1}{2} (g_1 + r_1 + g_2 + r_2) + \frac{1}{2} (g_1 r_2 + g_2 r_1 + r_1 r_2) $ $ - \frac{1}{4} (g_1 + g_2) (r_1 + r_2 + (g_1 + r_1) (g_2 + r_2)) $ $ - \frac{1}{8} (r_1 + r_2 + (g_1 + r_1) (g_2 + r_2))^{2} + r $ with $ \lvert r \rvert \leq \frac{1}{2} (g_1 + r_1 + g_2 + r_2 + (g_1 + r_1) (g_2 + r_2))^{3} $.  The assertion now follows by integrating (6.2.12) with respect to P  \end{document} 